wip: functional correctness of bignumQ

code/experimental/ed25519/Hacl.Spec.BignumQ.Mul.fst
@@ -4,76 +4,12 @@ open FStar.Mul
 open Lib.IntTypes
 
 module S = Spec.Ed25519
+module Lemmas = Hacl.Spec.BignumQ.Lemmas
+
+include Hacl.Spec.BignumQ.Definitions
+
 
 #reset-options "--z3rlimit 50 --max_fuel 0 --max_ifuel 0"
-
-let qelem5 = (uint64 & uint64 & uint64 & uint64 & uint64)
-let qelem_wide5 = (uint64 & uint64 & uint64 & uint64 & uint64 & uint64 & uint64 & uint64 & uint64 & uint64)
-let qelem_after_mul5 = (uint128 & uint128 & uint128 & uint128 & uint128 & uint128 & uint128 & uint128 & uint128)
-
-
-let scale64 = s:nat{s <= 256}
-let nat5 = (nat & nat & nat & nat & nat)
-
-let scale64_5 = x:nat5{let (x1,x2,x3,x4,x5) = x in
-		       x1 <= 256 /\ x2 <= 256 /\ x3 <= 256 /\ x4 <= 256 /\ x5 <= 256}
-
-abstract
-let pow56: (pow56: pos { pow2 64 == 256 * pow56 /\ pow2 128 == 65536 * pow56 * pow56 /\ pow56 == pow2 56 }) =
-  let pow56: pos = normalize_term (pow2 56) in
-  assert_norm (pow56 > 0);
-  assert_norm (pow56 == pow2 56);
-  assert_norm (pow2 64 == 256 * pow56);
-  assert_norm (pow2 128 == 65536 * pow56 * pow56);
-  pow56
-
-abstract
-let pow112: (pow112: pos { pow112 == pow2 112 /\ pow112 == pow56 * pow56}) =
-  let pow112: pos = normalize_term (pow2 112) in
-  assert_norm (pow112 > 0);
-  assert_norm (pow112 == pow2 112);
-  assert_norm (pow2 112 == pow2 56 * pow2 56);
-  pow112
-
-abstract
-let pow168: (pow168: pos { pow168 == pow2 168 /\ pow168 == pow56 * pow56 * pow56}) =
-  let pow168: pos = normalize_term (pow2 168) in
-  assert_norm (pow168 > 0);
-  assert_norm (pow168 == pow2 168);
-  assert_norm (pow2 168 == pow2 56 * pow2 56 * pow2 56);
-  pow168
-
-abstract
-let pow224: (pow224: pos { pow224 == pow2 224 /\ pow224 == pow56 * pow56 * pow56 * pow56}) =
-  let pow224: pos = normalize_term (pow2 224) in
-  assert_norm (pow224 > 0);
-  assert_norm (pow224 == pow2 224);
-  assert_norm (pow2 224 == pow2 56 * pow2 56 * pow2 56 * pow2 56);
-  pow224
-
-
-inline_for_extraction noextract
-let max56 = pow56 - 1
-
-let qelem_fits1 (x:uint64) (m:scale64) =
-  uint_v x <= m * max56
-
-let qelem_fits5 (f:qelem5) (m:scale64_5) =
-  let (x1,x2,x3,x4,x5) = f in
-  let (m1,m2,m3,m4,m5) = m in
-  qelem_fits1 x1 m1 /\
-  qelem_fits1 x2 m2 /\
-  qelem_fits1 x3 m3 /\
-  qelem_fits1 x4 m4 /\
-  qelem_fits1 x5 m5
-
-
-noextract
-val as_nat5: f:qelem5 -> GTot nat
-let as_nat5 f =
-  let (s0, s1, s2, s3, s4) = f in
-  v s0 + v s1 * pow56 + v s2 * pow112 + v s3 * pow168 + v s4 * pow224
-
 
 inline_for_extraction noextract
 let mask56 : x:uint64{v x == pow2 56 - 1} =
@@ -111,28 +47,6 @@ let make_mu m =
   (m0, m1, m2, m3, m4)
 
 
-val lemma_choose_step:
-    bit:uint64{v bit <= 1}
-  -> x:uint64
-  -> y:uint64
-  -> Lemma
-     (let mask = bit -. u64 1 in
-      let z = x ^. (mask &. (x ^. y)) in
-      if v bit = 1 then z == x else z == y)
-
-let lemma_choose_step bit p1 p2 =
-  let mask = bit -. u64 1 in
-  assert (v bit == 0 ==> v mask == pow2 64 - 1);
-  assert (v bit == 1 ==> v mask == 0);
-  let dummy = mask &. (p1 ^. p2) in
-  logand_lemma mask (p1 ^. p2);
-  assert (v bit == 1 ==> v dummy == 0);
-  assert (v bit == 0 ==> v dummy ==  v (p1 ^. p2));
-  let p1' = p1 ^. dummy in
-  assert (v dummy == v (if v bit = 1 then u64 0 else (p1 ^. p2)));
-  logxor_lemma p1 p2
-
-
 inline_for_extraction noextract
 val choose:
     b:uint64
@@ -145,15 +59,15 @@ val choose:
 let choose b (x0, x1, x2, x3, x4) (y0, y1, y2, y3, y4) =
   let mask = b -. u64 1 in
   let z0 = x0 ^. (mask &. (x0 ^. y0)) in
-  lemma_choose_step b x0 y0;
+  Lemmas.lemma_choose_step b x0 y0;
   let z1 = x1 ^. (mask &. (x1 ^. y1)) in
-  lemma_choose_step b x1 y1;
+  Lemmas.lemma_choose_step b x1 y1;
   let z2 = x2 ^. (mask &. (x2 ^. y2)) in
-  lemma_choose_step b x2 y2;
+  Lemmas.lemma_choose_step b x2 y2;
   let z3 = x3 ^. (mask &. (x3 ^. y3)) in
-  lemma_choose_step b x3 y3;
+  Lemmas.lemma_choose_step b x3 y3;
   let z4 = x4 ^. (mask &. (x4 ^. y4)) in
-  lemma_choose_step b x4 y4;
+  Lemmas.lemma_choose_step b x4 y4;
   (z0, z1, z2, z3, z4)
 
 
@@ -198,16 +112,23 @@ let subm_conditional (x0, x1, x2, x3, x4) =
   let (b4, t4) = subm_step x4 (y4 +! b3) in
   assert (v x4 - v y4 - v b3 == v t4 - v b4 * pow56);
 
+  Lemmas.lemma_subm_conditional
+    (v x0) (v x1) (v x2) (v x3) (v x4)
+    (v y0) (v y1) (v y2) (v y3) (v y4)
+    (v b0) (v b1) (v b2) (v b3) (v b4);
+
   assert (
     as_nat5 (t0, t1, t2, t3, t4) - v b4 * pow56 * pow224 ==
     as_nat5 (x0, x1, x2, x3, x4) - as_nat5 (y0, y1, y2, y3, y4));
 
-  assert_norm (pow56 * pow224 = pow2 280);
-  assert (as_nat5 (t0, t1, t2, t3, t4) - v b4 * pow2 280 == as_nat5 (x0, x1, x2, x3, x4) - S.q);
-  //assert (as_nat5 (x0, x1, x2, x3, x4) < pow2 280);
+  //assert_norm (pow56 * pow224 = pow2 280);
+  //assert (as_nat5 (t0, t1, t2, t3, t4) - v b4 * pow2 280 == as_nat5 (x0, x1, x2, x3, x4) - S.q);
+  Lemmas.lemma_as_nat5 (x0, x1, x2, x3, x4);
+  Lemmas.lemma_as_nat5 (t0, t1, t2, t3, t4);
+
   //assert (if v b4 = 0 then as_nat5 (x0, x1, x2, x3, x4) >= S.q else as_nat5 (x0, x1, x2, x3, x4) < S.q);
   assert (if as_nat5 (x0, x1, x2, x3, x4) >= S.q then v b4 == 0 else v b4 == 1);
-  //assert (qelem_fits5 (t0, t1, t2, t3, t4) (1, 1, 1, 1, 1));
+
   let (z0, z1, z2, z3, z4) = choose b4 (x0, x1, x2, x3, x4) (t0, t1, t2, t3, t4) in
   assert (
     if as_nat5 (x0, x1, x2, x3, x4) >= S.q
@@ -272,62 +193,37 @@ let add_modq5 (x0, x1, x2, x3, x4) (y0, y1, y2, y3, y4) =
 
 
 inline_for_extraction noextract
-val subm_last_step: x:uint64 -> y:uint64 -> uint64 & uint64
-let subm_last_step x y =
-  let b = (x -. y) >>. 63ul in
-  let t = (b <<. 40ul) +. x -. y in
-  b, t
+val carry56_wide: x:uint128 ->
+  Pure (uint128 & uint64)
+  (requires True) // v x < pow2 117 ==> v c < pow2 61
+  (ensures fun (c, t) -> v t < pow56 /\
+    v c * pow56 + v t == v x)
 
-
-inline_for_extraction noextract
-val sub_mod_264: x:qelem5 -> y:qelem5 -> z:qelem5
-let sub_mod_264 (x0, x1, x2, x3, x4) (y0, y1, y2, y3, y4) =
-  let (c1, t0) = subm_step x0 y0 in
-  let (c2, t1) = subm_step x1 (y1 +. c1) in
-  let (c3, t2) = subm_step x2 (y2 +. c2) in
-  let (c4, t3) = subm_step x3 (y3 +. c3) in
-  let (c5, t4) = subm_last_step x4 (y4 +. c4) in
-  (t0, t1, t2, t3, t4)
-
-
-inline_for_extraction noextract
-val carry56_wide: x:uint128 -> uint128 & uint64
 let carry56_wide x =
   let carry = x >>. 56ul in
   let t     = to_u64 x &. mask56 in
+  assert_norm (pow2 56 < pow2 64);
+  mod_mask_lemma (to_u64 x) 56ul;
+  assert (v (mod_mask #U64 #SEC 56ul) == v mask56);
+  assert (v t == (v x % pow2 64) % pow2 56);
+  FStar.Math.Lemmas.pow2_modulo_modulo_lemma_1 (v x) 56 64;
+  assert (v t == v x % pow2 56);
+  assert (v x == v carry * pow2 56 + v t);
   carry, t
 
 
 inline_for_extraction noextract
-val low_mul_5: x:qelem5 -> y:qelem5 -> z:qelem5
-let low_mul_5 (x0, x1, x2, x3, x4) (y0, y1, y2, y3, y4) =
-  let xy00 = mul64_wide x0 y0 in
-  let xy01 = mul64_wide x0 y1 in
-  let xy02 = mul64_wide x0 y2 in
-  let xy03 = mul64_wide x0 y3 in
-  let xy04 = mul64_wide x0 y4 in
-  let xy10 = mul64_wide x1 y0 in
-  let xy11 = mul64_wide x1 y1 in
-  let xy12 = mul64_wide x1 y2 in
-  let xy13 = mul64_wide x1 y3 in
-  let xy20 = mul64_wide x2 y0 in
-  let xy21 = mul64_wide x2 y1 in
-  let xy22 = mul64_wide x2 y2 in
-  let xy30 = mul64_wide x3 y0 in
-  let xy31 = mul64_wide x3 y1 in
-  let xy40 = mul64_wide x4 y0 in
+val mul_5:
+    x:qelem5
+  -> y:qelem5 ->
+  Pure qelem_wide5
+  (requires
+    qelem_fits5 x (1, 1, 1, 1, 1) /\
+    qelem_fits5 y (1, 1, 1, 1, 1))
+  (ensures fun r ->
+    qelem_wide_fits5 r (1, 1, 1, 1, 1, 1, 1, 1, 1, 1) /\
+    wide_as_nat5 r == as_nat5 x * as_nat5 y)
 
-
-  let (carry, t0) = carry56_wide xy00 in
-  let (carry, t1) = carry56_wide (xy01 +. xy10 +. carry) in
-  let (carry, t2) = carry56_wide (xy02 +. xy11 +. xy20 +. carry) in
-  let (carry, t3) = carry56_wide (xy03 +. xy12 +. xy21 +. xy30 +. carry) in
-  let t4 = to_u64 (xy04 +. xy13 +. xy22 +. xy31 +. xy40 +. carry) &. mask40 in
-  (t0, t1, t2, t3, t4)
-
-
-inline_for_extraction noextract
-val mul_5: x:qelem5 -> y:qelem5 -> z:qelem_after_mul5
 let mul_5 (x0, x1, x2, x3, x4) (y0, y1, y2, y3, y4) =
   let xy00 = mul64_wide x0 y0 in
   let xy01 = mul64_wide x0 y1 in
@@ -354,98 +250,226 @@ let mul_5 (x0, x1, x2, x3, x4) (y0, y1, y2, y3, y4) =
   let xy42 = mul64_wide x4 y2 in
   let xy43 = mul64_wide x4 y3 in
   let xy44 = mul64_wide x4 y4 in
-  let z0 = xy00 in
-  let z1 = xy01 +. xy10 in
-  let z2 = xy02 +. xy11 +. xy20 in
-  let z3 = xy03 +. xy12 +. xy21 +. xy30 in
-  let z4 = xy04 +. xy13 +. xy22 +. xy31 +. xy40 in
+  let z0 = xy00 in // < pow2 112
+  let z1 = xy01 +. xy10 in // < pow2 113
+  let z2 = xy02 +. xy11 +. xy20 in // < pow2 114
+  let z3 = xy03 +. xy12 +. xy21 +. xy30 in // < pow2 115
+  let z4 = xy04 +. xy13 +. xy22 +. xy31 +. xy40 in // < pow2 116
   let z5 =         xy14 +. xy23 +. xy32 +. xy41 in
   let z6 =                 xy24 +. xy33 +. xy42 in
   let z7 =                         xy34 +. xy43 in
   let z8 =                                 xy44 in
-  (z0, z1, z2, z3, z4, z5, z6, z7, z8)
+  //(z0, z1, z2, z3, z4, z5, z6, z7, z8)
 
-
-inline_for_extraction noextract
-val carry: qelem_after_mul5 -> qelem_wide5
-let carry (z0, z1, z2, z3, z4, z5, z6, z7, z8) =
-  let (carry, x0) = carry56_wide z0 in
-  let (carry, x1) = carry56_wide (z1 +. carry) in
-  let (carry, x2) = carry56_wide (z2 +. carry) in
-  let (carry, x3) = carry56_wide (z3 +. carry) in
-  let (carry, x4) = carry56_wide (z4 +. carry) in
-  let (carry, x5) = carry56_wide (z5 +. carry) in
-  let (carry, x6) = carry56_wide (z6 +. carry) in
-  let (carry, x7) = carry56_wide (z7 +. carry) in
-  let (carry, x8) = carry56_wide (z8 +. carry) in
-  let x9 = to_u64 carry in
+  let (c0, x0) = carry56_wide z0 in
+  let (c1, x1) = carry56_wide (z1 +. c0) in
+  let (c2, x2) = carry56_wide (z2 +. c1) in
+  let (c3, x3) = carry56_wide (z3 +. c2) in
+  let (c4, x4) = carry56_wide (z4 +. c3) in
+  let (c5, x5) = carry56_wide (z5 +. c4) in
+  let (c6, x6) = carry56_wide (z6 +. c5) in
+  let (c7, x7) = carry56_wide (z7 +. c6) in
+  let (c8, x8) = carry56_wide (z8 +. c7) in
+  let x9 = to_u64 c8 in admit();
   (x0, x1, x2, x3, x4, x5, x6, x7, x8, x9)
 
 
 inline_for_extraction noextract
-val mul_carry5: qelem5 -> qelem5 -> qelem_wide5
-let mul_carry5 (x0, x1, x2, x3, x4) (y0, y1, y2, y3, y4) =
-  let (z0, z1, z2, z3, z4, z5, z6, z7, z8) = mul_5 (x0, x1, x2, x3, x4) (y0, y1, y2, y3, y4) in
-  let (r0, r1, r2, r3, r4, r5, r6, r7, r8, r9) = carry (z0, z1, z2, z3, z4, z5, z6, z7, z8) in
-  (r0, r1, r2, r3, r4, r5, r6, r7, r8, r9)
+val low_mul_5:
+    x:qelem5
+  -> y:qelem5 ->
+  Pure qelem5
+  (requires
+    qelem_fits5 x (1, 1, 1, 1, 1) /\
+    qelem_fits5 y (1, 1, 1, 1, 1))
+  (ensures fun r ->
+    qelem_fits5 r (1, 1, 1, 1, 1) /\
+    as_nat5 r == (as_nat5 x * as_nat5 y) % pow2 264)
+
+let low_mul_5 (x0, x1, x2, x3, x4) (y0, y1, y2, y3, y4) =
+  let xy00 = mul64_wide x0 y0 in
+  let xy01 = mul64_wide x0 y1 in
+  let xy02 = mul64_wide x0 y2 in
+  let xy03 = mul64_wide x0 y3 in
+  let xy04 = mul64_wide x0 y4 in
+  let xy10 = mul64_wide x1 y0 in
+  let xy11 = mul64_wide x1 y1 in
+  let xy12 = mul64_wide x1 y2 in
+  let xy13 = mul64_wide x1 y3 in
+  let xy20 = mul64_wide x2 y0 in
+  let xy21 = mul64_wide x2 y1 in
+  let xy22 = mul64_wide x2 y2 in
+  let xy30 = mul64_wide x3 y0 in
+  let xy31 = mul64_wide x3 y1 in
+  let xy40 = mul64_wide x4 y0 in
+
+
+  let (c0, t0) = carry56_wide xy00 in
+  let (c1, t1) = carry56_wide (xy01 +. xy10 +. c0) in
+  let (c2, t2) = carry56_wide (xy02 +. xy11 +. xy20 +. c1) in
+  let (c3, t3) = carry56_wide (xy03 +. xy12 +. xy21 +. xy30 +. c2) in
+  let t4 = to_u64 (xy04 +. xy13 +. xy22 +. xy31 +. xy40 +. c3) &. mask40 in admit();
+  (t0, t1, t2, t3, t4)
 
 
 inline_for_extraction noextract
-val mod_264: qelem_wide5 -> qelem5
-let mod_264 (t0, t1, t2, t3, t4, t5, t6, t7, t8, t9) =
-  (t0, t1, t2, t3, t4 &. mask40)
+val div_2_24_step: x:uint64 -> y:uint64 ->
+  Pure uint64
+  (requires v x < pow56 /\ v y < pow56)
+  (ensures  fun r -> v r < pow56 /\
+    v r == v x / pow2 24 + pow2 32 * (v y % pow2 24))
 
-
-inline_for_extraction noextract
-val div_2_24_step: x:uint64 -> y:uint64 -> uint64
 let div_2_24_step x y =
   let y' = (y &. u64 0xffffff) <<. 32ul in
+  assert_norm (pow2 24 - 1 = 0xffffff);
+  assert_norm (pow2 24 < pow2 64);
+  mod_mask_lemma y 24ul;
+  assert (v (mod_mask #U64 #SEC 24ul) == 0xffffff);
+  assert (v (y &. u64 0xffffff) == v y % pow2 24);
+  assert (v y' == (v y % pow2 24) * pow2 32);
   let x' = x >>. 24ul in
-  let z = y' |. x' in
+  FStar.Math.Lemmas.pow2_minus 56 24;
+  assert (v x' < pow2 32);
+  let z = x' |. y' in
+  logor_disjoint x' y' 32;
+  assert (v z == v x / pow2 24 + pow2 32 * (v y % pow2 24));
   z
 
 
 inline_for_extraction noextract
-val div_248: qelem_wide5 -> qelem5
+val div_248: x:qelem_wide5 ->
+  Pure qelem5
+  (requires
+    qelem_wide_fits5 x (1, 1, 1, 1, 1, 1, 1, 1, 1, 1) /\
+    wide_as_nat5 x < pow2 512)
+  (ensures fun r ->
+    qelem_fits5 r (1, 1, 1, 1, 1) /\
+    as_nat5 r == (wide_as_nat5 x) / pow2 248)
+
 let div_248 (x0, x1, x2, x3, x4, x5, x6, x7, x8, x9) =
+  // x / pow2 248 == (x / pow2 224) / pow2 24
   let z0 = div_2_24_step x4 x5 in
   let z1 = div_2_24_step x5 x6 in
   let z2 = div_2_24_step x6 x7 in
   let z3 = div_2_24_step x7 x8 in
   let z4 = div_2_24_step x8 x9 in
+  assert (qelem_fits5 (z0, z1, z2, z3, z4) (1, 1, 1, 1, 1));
+  Lemmas.lemma_div248 (x0, x1, x2, x3, x4, x5, x6, x7, x8, x9);
   (z0, z1, z2, z3, z4)
 
 
 inline_for_extraction noextract
-val div_2_40_step: x:uint64 -> y:uint64 -> uint64
+val div_2_40_step: x:uint64 -> y:uint64 ->
+  Pure uint64
+  (requires v x < pow56)
+  (ensures  fun z -> v z < pow56 /\
+    v z == v x / pow2 40 + pow2 16 * (v y % pow2 40))
+
 let div_2_40_step x y =
   let y' = (y &. mask40) <<. 16ul in
+  assert_norm (pow2 40 < pow2 64);
+  mod_mask_lemma y 40ul;
+  assert (v (mod_mask #U64 #SEC 40ul) == v mask40);
+  assert (v y' == (v y % pow2 40) * pow2 16);
+
   let x' = x >>. 40ul in
-  let z = y' |. x' in
+  FStar.Math.Lemmas.pow2_minus 56 40;
+  assert (v x' == v x / pow2 40);
+  assert (v x' < pow2 16);
+  let z = x' |. y' in
+  logor_disjoint x' y' 16;
   z
 
 
 inline_for_extraction noextract
-val div_264: qelem_wide5 -> qelem5
+val div_264: x:qelem_wide5 ->
+  Pure qelem5
+  (requires
+    qelem_wide_fits5 x (1, 1, 1, 1, 1, 1, 1, 1, 1, 1))
+  (ensures fun z ->
+    qelem_fits5 z (1, 1, 1, 1, 1) /\
+    as_nat5 z == (wide_as_nat5 x) / pow2 264)
+
 let div_264 (x0, x1, x2, x3, x4, x5, x6, x7, x8, x9) =
   let z0 = div_2_40_step x4 x5 in
   let z1 = div_2_40_step x5 x6 in
   let z2 = div_2_40_step x6 x7 in
   let z3 = div_2_40_step x7 x8 in
   let z4 = div_2_40_step x8 x9 in
+  assert (qelem_fits5 (z0, z1, z2, z3, z4) (1, 1, 1, 1, 1));
+  admit();
   (z0, z1, z2, z3, z4)
+
+
+inline_for_extraction noextract
+val mod_264: t:qelem_wide5 ->
+  Pure qelem5
+  (requires
+    qelem_wide_fits5 t (1, 1, 1, 1, 1, 1, 1, 1, 1, 1))
+  (ensures fun r ->
+    qelem_fits5 r (1, 1, 1, 1, 1) /\
+    as_nat5 r == (wide_as_nat5 t) % pow2 264)
+
+let mod_264 (t0, t1, t2, t3, t4, t5, t6, t7, t8, t9) =
+  admit();
+  (t0, t1, t2, t3, t4 &. mask40)
+
+
+inline_for_extraction noextract
+val subm_last_step: x:uint64 -> y:uint64 ->
+  Pure (uint64 & uint64)
+  (requires v x < pow2 40 /\ v y <= pow2 40)
+  (ensures  fun (b, t) -> v b <= 1 /\ v t < pow2 40 /\
+    v x - v y == v t - pow2 40 * v b)
+
+let subm_last_step x y =
+  assert_norm (pow2 40 < pow2 63);
+  let b = (x -. y) >>. 63ul in
+  assert (if v x >= v y then v b == 0 else v b == 1);
+  let t = ((b <<. 40ul) +! x) -! y in
+  b, t
+
+
+inline_for_extraction noextract
+val sub_mod_264: x:qelem5 -> y:qelem5 ->
+  Pure qelem5
+  (requires
+    qelem_fits5 x (1, 1, 1, 1, 1) /\
+    qelem_fits5 y (1, 1, 1, 1, 1) /\
+    as_nat5 x < pow2 264 /\
+    as_nat5 y < pow2 264)
+  (ensures fun z ->
+    qelem_fits5 z (1, 1, 1, 1, 1) /\
+    as_nat5 z == (as_nat5 x - as_nat5 y) % pow2 264)
+
+let sub_mod_264 (x0, x1, x2, x3, x4) (y0, y1, y2, y3, y4) =
+  let (c1, t0) = subm_step x0 y0 in
+  let (c2, t1) = subm_step x1 (y1 +! c1) in
+  let (c3, t2) = subm_step x2 (y2 +! c2) in
+  let (c4, t3) = subm_step x3 (y3 +! c3) in
+  admit();
+  let (c5, t4) = subm_last_step x4 (y4 +! c4) in
+  (t0, t1, t2, t3, t4)
 
 
 // A = t, L = make_m()
 // b = 2^8, k = 32, mu = b^{2*k} / L = make_mu()
 inline_for_extraction noextract
-val barrett_reduction5: t:qelem_wide5 -> z:qelem5
+val barrett_reduction5: t:qelem_wide5 ->
+  Pure qelem5
+  (requires
+    qelem_wide_fits5 t (1, 1, 1, 1, 1, 1, 1, 1, 1, 1) /\
+    wide_as_nat5 t < pow2 512)
+  (ensures  fun z ->
+    qelem_fits5 z (1, 1, 1, 1, 1) /\
+    as_nat5 z == (wide_as_nat5 t) % S.q)
+
 let barrett_reduction5 (t0, t1, t2, t3, t4, t5, t6, t7, t8, t9) =
   let (m0, m1, m2, m3, m4) = make_m () in
   let (mu0, mu1, mu2, mu3, mu4) = make_mu () in
 
   let (q0, q1, q2, q3, q4) = div_248 (t0, t1, t2, t3, t4, t5, t6, t7, t8, t9) in
-  let (qmu0', qmu1', qmu2', qmu3', qmu4', qmu5', qmu6', qmu7', qmu8', qmu9') = mul_carry5 (q0, q1, q2, q3, q4) (mu0, mu1, mu2, mu3, mu4) in
+  let (qmu0', qmu1', qmu2', qmu3', qmu4', qmu5', qmu6', qmu7', qmu8', qmu9') = mul_5 (q0, q1, q2, q3, q4) (mu0, mu1, mu2, mu3, mu4) in
   let (qdiv0, qdiv1, qdiv2, qdiv3, qdiv4) = div_264 (qmu0', qmu1', qmu2', qmu3', qmu4', qmu5', qmu6', qmu7', qmu8', qmu9') in
   //u = qdiv == (A / b^{k-1}) * mu / b^{k+1} == ((A / 2^248) * mu) / 2^264
 
@@ -459,12 +483,25 @@ let barrett_reduction5 (t0, t1, t2, t3, t4, t5, t6, t7, t8, t9) =
   //u == s == (r - v) mod b^{k+1} == (r - v) mod 2^264
 
   let (o0, o1, o2, o3, o4) = subm_conditional (s0, s1, s2, s3, s4) in
+  admit();
   (o0, o1, o2, o3, o4)
 
 
 inline_for_extraction noextract
-val mul_modq5: qelem5 -> qelem5 -> qelem5
+val mul_modq5: x:qelem5 -> y:qelem5 ->
+  Pure qelem5
+  (requires
+    qelem_fits5 x (1, 1, 1, 1, 1) /\
+    qelem_fits5 y (1, 1, 1, 1, 1) /\
+    as_nat5 x < pow2 256 /\
+    as_nat5 y < pow2 256)
+  (ensures  fun r ->
+    qelem_fits5 r (1, 1, 1, 1, 1) /\
+    as_nat5 r == (as_nat5 x * as_nat5 y) % S.q)
+
 let mul_modq5 (x0, x1, x2, x3, x4) (y0, y1, y2, y3, y4) =
-  let (r0, r1, r2, r3, r4, r5, r6, r7, r8, r9) = mul_carry5 (x0, x1, x2, x3, x4) (y0, y1, y2, y3, y4) in
+  let (r0, r1, r2, r3, r4, r5, r6, r7, r8, r9) = mul_5 (x0, x1, x2, x3, x4) (y0, y1, y2, y3, y4) in
+  Lemmas.lemma_mul_lt (as_nat5 (x0, x1, x2, x3, x4)) (pow2 256) (as_nat5 (y0, y1, y2, y3, y4)) (pow2 256);
+  assert_norm (pow2 256 * pow2 256 = pow2 512);
   let (o0, o1, o2, o3, o4) = barrett_reduction5 (r0, r1, r2, r3, r4, r5, r6, r7, r8, r9) in
   (o0, o1, o2, o3, o4)
