code/experimental/ed25519/Hacl.Spec.BignumQ.Lemmas.fst
@@ -1,0 +1,244 @@
+module Hacl.Spec.BignumQ.Lemmas
+
+open FStar.Mul
+open Lib.IntTypes
+
+include Hacl.Spec.BignumQ.Definitions
+
+#reset-options "--z3rlimit 50 --max_fuel 0 --max_ifuel 0"
+
+val lemma_mul_lt:a:nat -> b:nat -> c:nat -> d:nat ->
+  Lemma
+  (requires a < b /\ c < d)
+  (ensures  a * c < b * d)
+
+let lemma_mul_lt a b c d = ()
+
+
+val lemma_as_nat5: f:qelem5 ->
+  Lemma
+  (requires qelem_fits5 f (1, 1, 1, 1, 1))
+  (ensures  as_nat5 f < pow2 280)
+
+let lemma_as_nat5 f =
+  //let (f0, f1, f2, f3, f4) = f in
+  //assert (as_nat5 f == v f0 + v f1 * pow56 + v f2 * pow112 + v f3 * pow168 + v f4 * pow224);
+  assert_norm (pow2 56 * pow2 56 = pow2 112);
+  assert_norm (pow2 56 * pow2 112 = pow2 168);
+  assert_norm (pow2 56 * pow2 168 = pow2 224);
+  assert_norm (pow2 56 * pow2 224 = pow2 280)
+
+
+val lemma_choose_step:
+    bit:uint64{v bit <= 1}
+  -> x:uint64
+  -> y:uint64
+  -> Lemma
+     (let mask = bit -. u64 1 in
+      let z = x ^. (mask &. (x ^. y)) in
+      if v bit = 1 then z == x else z == y)
+
+let lemma_choose_step bit p1 p2 =
+  let mask = bit -. u64 1 in
+  assert (v bit == 0 ==> v mask == pow2 64 - 1);
+  assert (v bit == 1 ==> v mask == 0);
+  let dummy = mask &. (p1 ^. p2) in
+  logand_lemma mask (p1 ^. p2);
+  assert (v bit == 1 ==> v dummy == 0);
+  assert (v bit == 0 ==> v dummy ==  v (p1 ^. p2));
+  let p1' = p1 ^. dummy in
+  assert (v dummy == v (if v bit = 1 then u64 0 else (p1 ^. p2)));
+  logxor_lemma p1 p2
+
+
+val lemma_subm_conditional:
+    x0:nat -> x1:nat -> x2:nat -> x3:nat -> x4:nat
+  -> y0:nat -> y1:nat -> y2:nat -> y3:nat -> y4:nat
+  -> b0:nat -> b1:nat -> b2:nat -> b3:nat -> b4:nat ->
+  Lemma (
+    x0 - y0 + b0 * pow2 56 +
+    (x1 - y1 - b0 + b1 * pow2 56) * pow2 56 +
+    (x2 - y2 - b1 + b2 * pow2 56) * pow2 112 +
+    (x3 - y3 - b2 + b3 * pow2 56) * pow2 168 +
+    (x4 - y4 - b3 + b4 * pow2 56) * pow2 224 ==
+    (x0 + x1 * pow2 56 + x2 * pow2 112 + x3 * pow2 168 + x4 * pow2 224) -
+    (y0 + y1 * pow2 56 + y2 * pow2 112 + y3 * pow2 168 + y4 * pow2 224) + b4 * pow2 280)
+
+let lemma_subm_conditional x0 x1 x2 x3 x4 y0 y1 y2 y3 y4 b0 b1 b2 b3 b4 =
+  assert_norm (pow2 56 * pow2 56 = pow2 112);
+  assert_norm (pow2 56 * pow2 112 = pow2 168);
+  assert_norm (pow2 56 * pow2 168 = pow2 224);
+  assert_norm (pow2 56 * pow2 224 = pow2 280)
+
+
+val lemma_div224: x:qelem_wide5 ->
+  Lemma
+  (requires
+    qelem_wide_fits5 x (1, 1, 1, 1, 1, 1, 1, 1, 1, 1) /\
+    wide_as_nat5 x < pow2 512)
+  (ensures
+   (let (x0, x1, x2, x3, x4, x5, x6, x7, x8, x9) = x in
+    wide_as_nat5 x / pow2 224 ==
+    v x4 + v x5 * pow2 56 + v x6 * pow2 112 + v x7 * pow2 168 + v x8 * pow2 224 + v x9 * pow2 280))
+
+let lemma_div224 x =
+  let (x0, x1, x2, x3, x4, x5, x6, x7, x8, x9) = x in
+  assert
+    (wide_as_nat5 x ==
+     v x0 + v x1 * pow2 56 + v x2 * pow2 112 + v x3 * pow2 168 + v x4 * pow2 224 +
+     v x5 * pow2 280 + v x6 * pow2 336 + v x7 * pow2 392 + v x8 * pow2 448 + v x9 * pow2 504);
+  assert_norm (pow2 56 * pow2 224 == pow2 280);
+  assert_norm (pow2 112 * pow2 224 == pow2 336);
+  assert_norm (pow2 168 * pow2 224 == pow2 392);
+  assert_norm (pow2 224 * pow2 224 == pow2 448);
+  assert_norm (pow2 280 * pow2 224 == pow2 504);
+  let open FStar.Calc in
+  calc (==) {
+    wide_as_nat5 x / pow2 224;
+    (==) { }
+    (v x0 + v x1 * pow2 56 + v x2 * pow2 112 + v x3 * pow2 168 +
+    (v x4 + v x5 * pow2 56 + v x6 * pow2 112 + v x7 * pow2 168 + v x8 * pow2 224 + v x9 * pow2 280) * pow2 224) / pow2 224;
+    (==) {
+      FStar.Math.Lemmas.lemma_div_plus
+	(v x0 + v x1 * pow2 56 + v x2 * pow2 112 + v x3 * pow2 168)
+	(v x4 + v x5 * pow2 56 + v x6 * pow2 112 + v x7 * pow2 168 + v x8 * pow2 224 + v x9 * pow2 280) (pow2 224) }
+    (v x0 + v x1 * pow2 56 + v x2 * pow2 112 + v x3 * pow2 168) / pow2 224 +
+    v x4 + v x5 * pow2 56 + v x6 * pow2 112 + v x7 * pow2 168 + v x8 * pow2 224 + v x9 * pow2 280;
+    (==) { FStar.Math.Lemmas.small_division_lemma_1 (v x0 + v x1 * pow2 56 + v x2 * pow2 112 + v x3 * pow2 168) (pow2 224) }
+      v x4 + v x5 * pow2 56 + v x6 * pow2 112 + v x7 * pow2 168 + v x8 * pow2 224 + v x9 * pow2 280;
+    }
+
+
+#set-options "--z3rlimit 100"
+
+val lemma_div248_aux: x:qelem_wide5 ->
+  Lemma
+  (requires
+    qelem_wide_fits5 x (1, 1, 1, 1, 1, 1, 1, 1, 1, 1) /\
+    wide_as_nat5 x < pow2 512)
+  (ensures
+   (let (x0, x1, x2, x3, x4, x5, x6, x7, x8, x9) = x in
+    wide_as_nat5 x / pow2 248 ==
+      v x4 / pow2 24 + v x5 * pow2 32 + v x6 * pow2 88 + v x7 * pow2 144 + v x8 * pow2 200 + v x9 * pow2 256))
+
+let lemma_div248_aux x =
+  let (x0, x1, x2, x3, x4, x5, x6, x7, x8, x9) = x in
+  assert_norm (pow2 248 == pow2 224 * pow2 24);
+  assert_norm (pow2 56 == pow2 32 * pow2 24);
+  assert_norm (pow2 112 == pow2 88 * pow2 24);
+  assert_norm (pow2 168 == pow2 144 * pow2 24);
+  assert_norm (pow2 224 == pow2 200 * pow2 24);
+  assert_norm (pow2 280 == pow2 256 * pow2 24);
+  assert_norm (0 < pow2 24);
+
+  calc (==) {
+    wide_as_nat5 x / pow2 248;
+  (==) { FStar.Math.Lemmas.division_multiplication_lemma (wide_as_nat5 x) (pow2 224) (pow2 24) }
+    (wide_as_nat5 x / pow2 224) / pow2 24;
+  (==) { lemma_div224 x }
+    (v x4 + v x5 * pow2 56 + v x6 * pow2 112 + v x7 * pow2 168 + v x8 * pow2 224 + v x9 * pow2 280) / pow2 24;
+  (==) { }
+    (v x4 + (v x5 * pow2 32 + v x6 * pow2 88 + v x7 * pow2 144 + v x8 * pow2 200 + v x9 * pow2 256) * pow2 24) / pow2 24;
+  (==) { FStar.Math.Lemmas.lemma_div_plus (v x4) (v x5 * pow2 32 + v x6 * pow2 88 + v x7 * pow2 144 + v x8 * pow2 200 + v x9 * pow2 256) (pow2 24) }
+    v x4 / pow2 24 + v x5 * pow2 32 + v x6 * pow2 88 + v x7 * pow2 144 + v x8 * pow2 200 + v x9 * pow2 256;
+  }
+
+
+val lemma_div248_x5: x5:uint64 ->
+  Lemma ( pow2 32 * (v x5 % pow2 24) + v x5 / pow2 24 * pow2 56 == v x5 * pow2 32)
+let lemma_div248_x5 x5 =
+  assert_norm (pow2 32 * pow2 24 = pow2 56)
+
+val lemma_div248_x6: x6:uint64 ->
+  Lemma (pow2 32 * (v x6 % pow2 24) * pow2 56 + v x6 / pow2 24 * pow2 112 == v x6 * pow2 88)
+let lemma_div248_x6 x6 =
+  calc (==) {
+    pow2 32 * (v x6 % pow2 24) * pow2 56 + v x6 / pow2 24 * pow2 112;
+    (==) { assert_norm (pow2 32 * pow2 56 = pow2 88) }
+    (v x6 % pow2 24) * pow2 88 + v x6 / pow2 24 * pow2 112;
+    (==) { assert_norm (pow2 112 == pow2 88 * pow2 24) }
+    (v x6 % pow2 24) * pow2 88 + v x6 / pow2 24 * pow2 24 * pow2 88;
+    (==) { }
+    v x6 * pow2 88;
+    }
+
+val lemma_div248_x7: x7:uint64 ->
+  Lemma (pow2 32 * (v x7 % pow2 24) * pow2 112 + v x7 / pow2 24 * pow2 168 == v x7 * pow2 144)
+let lemma_div248_x7 x7 =
+  assert_norm (pow2 32 * pow2 112 = pow2 144);
+  assert_norm (pow2 168 == pow2 144 * pow2 24)
+
+val lemma_div248_x8: x8:uint64 ->
+  Lemma (pow2 32 * (v x8 % pow2 24) * pow2 168 + v x8 / pow2 24 * pow2 224 == v x8 * pow2 200)
+let lemma_div248_x8 x8 =
+  assert_norm (pow2 32 * pow2 168 = pow2 200);
+  assert_norm (pow2 224 == pow2 200 * pow2 24)
+
+val lemma_div248_x9: x9:uint64{v x9 < pow2 24} ->
+  Lemma (pow2 32 * (v x9 % pow2 24) * pow2 224 == v x9 * pow2 256)
+let lemma_div248_x9 x9 =
+  assert_norm (pow2 32 * pow2 224 = pow2 256)
+
+val lemma_wide_as_nat_pow512: x:qelem_wide5 ->
+  Lemma
+  (requires
+    qelem_wide_fits5 x (1, 1, 1, 1, 1, 1, 1, 1, 1, 1) /\
+    wide_as_nat5 x < pow2 512)
+  (ensures
+   (let (x0, x1, x2, x3, x4, x5, x6, x7, x8, x9) = x in
+    v x9 < pow2 24))
+
+let lemma_wide_as_nat_pow512 x =
+  let (x0, x1, x2, x3, x4, x5, x6, x7, x8, x9) = x in
+  assert_norm (pow2 504 * pow2 8 = pow2 512);
+  FStar.Math.Lemmas.pow2_minus 512 504;
+  assert (v x9 < pow2 8);
+  assert_norm (pow2 8 < pow2 24)
+
+
+val lemma_div248: x:qelem_wide5 ->
+  Lemma
+  (requires
+    qelem_wide_fits5 x (1, 1, 1, 1, 1, 1, 1, 1, 1, 1) /\
+    wide_as_nat5 x < pow2 512)
+  (ensures
+   (let (x0, x1, x2, x3, x4, x5, x6, x7, x8, x9) = x in
+    let z0 = v x4 / pow2 24 + pow2 32 * (v x5 % pow2 24) in
+    let z1 = v x5 / pow2 24 + pow2 32 * (v x6 % pow2 24) in
+    let z2 = v x6 / pow2 24 + pow2 32 * (v x7 % pow2 24) in
+    let z3 = v x7 / pow2 24 + pow2 32 * (v x8 % pow2 24) in
+    let z4 = v x8 / pow2 24 + pow2 32 * (v x9 % pow2 24) in
+
+    wide_as_nat5 x / pow2 248 == z0 + z1 * pow2 56 + z2 * pow2 112 + z3 * pow2 168 + z4 * pow2 224))
+
+let lemma_div248 x =
+  let (x0, x1, x2, x3, x4, x5, x6, x7, x8, x9) = x in
+  lemma_wide_as_nat_pow512 x;
+  assert (v x9 < pow2 24);
+  let z0 = v x4 / pow2 24 + pow2 32 * (v x5 % pow2 24) in
+  let z1 = v x5 / pow2 24 + pow2 32 * (v x6 % pow2 24) in
+  let z2 = v x6 / pow2 24 + pow2 32 * (v x7 % pow2 24) in
+  let z3 = v x7 / pow2 24 + pow2 32 * (v x8 % pow2 24) in
+  let z4 = v x8 / pow2 24 + pow2 32 * (v x9 % pow2 24) in
+
+  calc (==) {
+    z0 + z1 * pow2 56 + z2 * pow2 112 + z3 * pow2 168 + z4 * pow2 224;
+  (==) { }
+    v x4 / pow2 24 + pow2 32 * (v x5 % pow2 24) +
+    v x5 / pow2 24 * pow2 56 + pow2 32 * (v x6 % pow2 24) * pow2 56 +
+    v x6 / pow2 24 * pow2 112 + pow2 32 * (v x7 % pow2 24) * pow2 112 +
+    v x7 / pow2 24 * pow2 168 + pow2 32 * (v x8 % pow2 24) * pow2 168 +
+    v x8 / pow2 24 * pow2 224 + pow2 32 * (v x9 % pow2 24) * pow2 224;
+  (==) { lemma_div248_x5 x5; lemma_div248_x6 x6 }
+    v x4 / pow2 24 + v x5 * pow2 32 + v x6 * pow2 88 +
+    pow2 32 * (v x7 % pow2 24) * pow2 112 +
+    v x7 / pow2 24 * pow2 168 + pow2 32 * (v x8 % pow2 24) * pow2 168 +
+    v x8 / pow2 24 * pow2 224 + pow2 32 * (v x9 % pow2 24) * pow2 224;
+  (==) { lemma_div248_x7 x7; lemma_div248_x8 x8 }
+    v x4 / pow2 24 + v x5 * pow2 32 + v x6 * pow2 88 + v x7 * pow2 144 + v x8 * pow2 200 +
+    pow2 32 * (v x9 % pow2 24) * pow2 224;
+  (==) { lemma_div248_x9 x9 }
+    v x4 / pow2 24 + v x5 * pow2 32 + v x6 * pow2 88 + v x7 * pow2 144 + v x8 * pow2 200 + v x9 * pow2 256;
+  (==) { lemma_div248_aux x }
+    wide_as_nat5 x / pow2 248;
+  }
